\begin{answer}
\begin{align*}
\ell_\text{semi-sup}(\theta^{(t+1)})
&= \alpha \ell_\text{sup}(\theta^{(t+1)}) + \ell_\text{unsup}(\theta^{(t+1)})
    &\text{Definition} \\
&\ge \alpha \ell_\text{sup}(\theta^{(t+1)}) + \sum_{i=1}^\nexp\sum_{\zsi}Q_i^{(t)}(\zsi)\log\frac{p(\xsi,\zsi;\theta^{(t+1)})}{Q_i^{(t)}(\zsi)}
    &\text{Jensen's inequality} \\
&\ge \alpha \ell_\text{sup}(\theta^{(t)}) + \sum_{i=1}^\nexp\sum_{\zsi}Q_i^{(t)}(\zsi)\log\frac{p(\xsi,\zsi;\theta^{(t)})}{Q_i^{(t)}(\zsi)}
    &\text{M-step} \\
&= \alpha \ell_\text{sup}(\theta^{(t)}) + \sum_{i=1}^\nexp\sum_{\zsi}Q_i^{(t)}(\zsi)\log\frac{p(\zsi|\xsi;\theta^{(t)})p(\xsi;\theta^{(t)})}{Q_i^{(t)}(\zsi)}
	&\text{Conditional probability} \\
&= \alpha \ell_\text{sup}(\theta^{(t)}) + \sum_{i=1}^\nexp\sum_{\zsi}Q_i^{(t)}(\zsi)\log p(\xsi;\theta^{(t)})
	&{Q^{(t)}(z) := p(z|x;\theta^{(t)})} \\
&= \alpha \ell_\text{sup}(\theta^{(t)}) + \ell_\text{unsup}(\theta^{(t)})
    &\sum_{\zsi}Q_i^{(t)}(\zsi)=1\\
&= \ell_\text{semi-sup}(\theta^{(t)})
\end{align*}
\end{answer}
