\begin{answer}
\allowdisplaybreaks

In order to simplify derivation, we denote $$w_j^{(i)} = Q^{(t)}_i(\zsi=j),$$ and $$\tilde{w}_j^{(i)} = \begin{cases} \alpha & \tilde{z}^{(i)} = j \\ 0 & \text{ otherwise.} \end{cases}$$

We further denote $S = \Sigma^{-1}$, and note that because of chain rule of calculus, $\nabla_S\ell = 0 \Rightarrow \nabla_\Sigma \ell = 0$. So we choose to rewrite the M-step in terms of $S$ and maximize it w.r.t $S$, and re-express the resulting solution back in terms of $\Sigma$.

Based on this, the M-step becomes:
\begin{align*}
\phi^{(t+1)}, \mu^{(t+1)}, S^{(t+1)} &=  \arg\max_{\phi,\mu,S} \sum_{i=1}^\nexp \sum_{j=1}^k Q_i^{(t)}(\zsi) \log \frac{p(\xsi,\zsi;\phi,\mu,S)}{Q_i^{(t)}(\zsi)} + \sum_{i=1}^{\tilde{\nexp}} \log p(\tilde{\xsi}, \tilde{\zsi}; \phi, \mu, S)\\
&=\arg\max_{\phi, \mu, S} \sum_{i=1}^\nexp \sum_{j=1}^k w^{(i)}_j \log \frac{ \frac{|S_j|^{1/2}}{(2\pi)^{\di/2}} \exp\left(-\frac{1}{2}(\xsi-\mu_j)^TS_j(\xsi-\mu_j)\right) \phi_j}{w^{(i)}_j } \\
&\quad\quad\quad +\sum_{i=1}^{\tilde{\nexp}} \sum_{j=1}^k \tilde{w}^{(i)}_j \log \frac{ \frac{|S_j|^{1/2}}{(2\pi)^{\di/2}} \exp\left(-\frac{1}{2}(\tilde{x}^{(i)}-\mu_j)^TS_j(\tilde{x}^{(i)}-\mu_j)\right) \phi_j}{\tilde{w}^{(i)}_j } \\
\end{align*}

First we start by maximizing w.r.t $\phi_j$. We construct the Lagrangian including the constraint that $\sum_{j=1}^k \phi_j = 1$, and absorbing all irrelevant terms into constant $C$:
\begin{align*}
\mathcal{L}(\phi, \beta) &= C + \sum_{i=1}^\nexp\sum_{j=1}^k w^{(i)}_j \log \phi_j + \sum_{i=1}^{\tilde{\nexp}}\sum_{j=1}^k \tilde{w}^{(i)}_j \log \phi_j + \beta\left(\sum_{j=1}^k \phi_j - 1\right) \\
\nabla_{\phi_j}\mathcal{L}(\phi, \beta) &=  \sum_{i=1}^\nexp w^{(i)}_j\frac{1}{\phi_j} + \sum_{i=1}^{\tilde{\nexp}} \tilde{w}^{(i)}_j\frac{1}{\phi_j} + \beta = 0 \\
&\Rightarrow \phi_j = \frac{\sum_{i=1}^\nexp w^{(i)}_j + \sum_{i=1}^{\tilde{\nexp}} \tilde{w}^{(i)}_j}{-\beta} \\
\nabla_\beta\mathcal{L}(\phi,\beta) &= \sum_{j=1}^k \phi_j -1 = 0 \\
&\Rightarrow \sum_{j=1}^k \frac{\sum_{i=1}^\nexp w^{(i)}_j + \sum_{i=1}^{\tilde{\nexp}} \tilde{w}^{(i)}_j}{-\beta} = 1 \\
&\Rightarrow -\beta = \sum_{j=1}^k \left(\sum_{i=1}^\nexp w^{(i)}_j + \sum_{i=1}^{\tilde{\nexp}} \tilde{w}^{(i)}_j\right)  \\
\Rightarrow \phi_j^{(t+1)} &= \frac{ \sum_{i=1}^\nexp w_j^{(i)} + \sum_{i=1}^{\tilde{\nexp}}\tilde{w}_j^{(i)}} { \sum_{j=1}^k \left(\sum_{i=1}^\nexp w^{(i)}_j + \sum_{i=1}^{\tilde{\nexp}} \tilde{w}^{(i)}_j\right) } \\
&= \frac{ \sum_{i=1}^\nexp w_j^{(i)} + \sum_{i=1}^{\tilde{\nexp}}\tilde{w}_j^{(i)}} { \nexp + \alpha \tilde{\nexp}}
\end{align*}

Next we derive the update for $\mu_j$ (absorbing irrelevant constants into $C$):
\begin{align*}
0 &= \nabla_{\mu_j} \left(\ldots\right) \\
&= -\nabla_{\mu_j} \left( C + \sum_{i=1}^\nexp w^{(i)}_j (\xsi-\mu_j)^TS_j(\xsi-\mu_j) + \sum_{i=1}^{\tilde{\nexp}} \tilde{w}^{(i)}_j (\tilde{x}^{(i)}-\mu_j)^TS_j(\tilde{x}^{(i)}-\mu_j)\right) \\
&= -\nabla_{\mu_j} \left(\sum_{i=1}^\nexp w^{(i)}_j (-2x^{(i)T} S\mu_j + \mu_j^TS_j\mu_j) + \sum_{i=1}^{\tilde{\nexp}} \tilde{w}^{(i)}_j (-2\tilde{x}^{(i)T}S\mu_j + \mu_j^TS_j\mu_j) \right) \\
&= - 2\left(\sum_{i=1}^\nexp w^{(i)}_j (-S\xsi + S\mu_j) + \sum_{i=1}^{\tilde{\nexp}} \tilde{w}^{(i)}_j (-S\tilde{x}^{(i)} + S\mu_j) \right) \\
&= 2S\left(\sum_{i=1}^\nexp w^{(i)}_j\xsi + \sum_{i=1}^{\tilde{\nexp}}\tilde{w}^{(i)}_j \tilde{x}^{(i)}\right) -2S\left(\sum_{i=1}^\nexp w^{(i)}_j + \sum_{i=1}^{\tilde{\nexp}} \tilde{w}^{(i)}_j \right)\mu_j \\
\Rightarrow \mu_j^{(t+1)} &= \frac{\sum_{i=1}^\nexp w_j^{(i)}\xsi + \sum_{i=1}^{\tilde{\nexp}}\tilde{w}^{(i)}_j \tilde{x}^{(i)}   }{ \sum_{i=1}^\nexp w_j^{(i)} + \sum_{i=1}^{\tilde{\nexp}}\tilde{w}^{(i)}_j }
\end{align*}

Finally we derive the update for $\Sigma_j$ via $S_j$:
\begin{align*}
0 &= \nabla_{S_j} \left(\ldots\right) \\
&= \nabla_{S_j} \left(C + \sum_{i=1}^\nexp w^{(i)}_j\left(\log |S_j| - (\xsi-\mu_j)^TS_j(\xsi-\mu_j)\right) + \sum_{i=1}^{\tilde{\nexp}} \tilde{w}^{(i)}_j\left(\log |S_j| - (\tilde{x}^{(i)}-\mu_j)^TS_j(\tilde{x}^{(i)}-\mu_j)\right)\right) \\
&= \sum_{i=1}^\nexp w^{(i)}_j\left(S_j^{-1} - (\xsi-\mu_j)(\xsi-\mu_j)^T\right) + \sum_{i=1}^{\tilde{\nexp}} \tilde{w}^{(i)}_j\left(S_j^{-1} - (\tilde{x}^{(i)}-\mu_j)(\tilde{x}^{(i)}-\mu_j)^T\right) \\
&= \left(\sum_{i=1}^\nexp w^{(i)}_j + \sum_{i=1}^{\tilde{\nexp}} \tilde{w}^{(i)}_j\right) S_j^{-1} - \left(\sum_{i=1}^\nexp w_{j}^{(i)}(\xsi-\mu_j)(\xsi-\mu_j)^T + \sum_{i=1}^{\tilde{\nexp}} \tilde{w}^{(i)}_j(\tilde{x}^{(i)} - \mu_j)(\tilde{x}^{(i)}-\mu_j)^T\right) \\
&\Rightarrow \Sigma_j^{(t+1)} = \frac{\sum_{i=1}^\nexp w_{j}^{(i)}(\xsi-\mu_j)(\xsi-\mu_j)^T + \sum_{i=1}^{\tilde{\nexp}} \tilde{w}^{(i)}_j(\tilde{x}^{(i)} - \mu_j)(\tilde{x}^{(i)}-\mu_j)^T}{\sum_{i=1}^\nexp w^{(i)}_j + \sum_{i=1}^{\tilde{\nexp}} \tilde{w}^{(i)}_j}
\end{align*}

This results in the final set of update expressions:
\begin{align*}
  \phi_j & := \frac{ \sum_{i=1}^\nexp w^{(i)}_j + \alpha \sum_{i=1}^{\tilde{\nexp}}\textbf{1}\{\tilde{z}^{(i)} = j\}}{\nexp + \alpha \tilde{\nexp}} \\
  \mu_j & := \frac{ \sum_{i=1}^\nexp w^{(i)}_j\xsi + \alpha\sum_{i=1}^{\tilde{\nexp}} \textbf{1}\{\tilde{z}^{(i)} = j\}\tilde{x}^{(i)}} {\sum_{i=1}^\nexp w^{(i)}_j + \alpha\sum_{i=1}^{\tilde{\nexp}} \textbf{1}\{\tilde{z}^{(i)} = j\} } \\
  \Sigma_j & := \frac{ \sum_{i=1}^\nexp w^{(i)}_j(\xsi-\mu_j)(\xsi-\mu_j)^T + \alpha\sum_{i=1}^{\tilde{\nexp}} \textbf{1}\{\tilde{z}^{(i)} = j\}(\tilde{x}^{(i)}-\mu_j)(\tilde{x}^{(i)}-\mu_j)^T} {\sum_{i=1}^\nexp w^{(i)}_j + \alpha\sum_{i=1}^{\tilde{\nexp}} \textbf{1}\{\tilde{z}^{(i)} = j\} }
\end{align*}
\end{answer}
