\begin{answer}

First, we have
\begin{align*}
\vec{y} &= X\theta + \vec{\epsilon},
    \quad \vec{\epsilon} \sim \mathcal{N}(0, \sigma^2I),
    \quad \theta \in \Re^{\di} \\
\Rightarrow \vec{y} &\sim \mathcal{N}(X\theta, \sigma^2I).
\end{align*}

Now,
\begin{align*}
\theta_{\text{MAP}} &= \arg\min_\theta - \log p(\vec{y}|X, \theta) + \frac{1}{2 \eta^2} ||\theta||_2^2 \\
&= \arg\min_\theta -\log \left(\frac{1}{\sqrt{(2\pi)^{\di} |\sigma^2I|}}\exp\left[-\frac{1}{2} (\vec{y} - X\theta)^T (\sigma^2 I)^{-1} (\vec{y} - X\theta) \right]\right) + \frac{1}{2 \eta^2}||\theta||_2^2 \\
&= \arg\min_\theta -C + \frac{1}{2 \sigma^2} (\vec{y} - X\theta)^T (\vec{y} - X\theta) + \frac{1}{2 \eta^2}||\theta||_2^2 \\
&= \arg\min_\theta ||X\theta - \vec{y}||_2^2 + \frac{\sigma^2}{\eta^2}||\theta||_2^2
\end{align*}

Let
\begin{align*}
J(\theta) &= ||X\theta - \vec{y}||_2^2 + \frac{\sigma^2}{\eta^2} ||\theta||_2^2 \\
&= (X\theta - \vec{y})^T(X\theta - \vec{y}) + \frac{\sigma^2}{\eta^2} ||\theta||_2^2 \\
\Rightarrow \nabla_\theta J(\theta) &= 2X^TX\theta - 2X^T\vec{y} + 2\frac{\sigma^2}{\eta^2} \theta \\
&= 2(X^TX + \frac{\sigma^2}{\eta^2}I)\theta - 2X^T\vec{y} = 0 \\
& \Rightarrow \boxed{\theta_\text{MAP} = \left(X^TX + \frac{\sigma^2}{\eta^2}I\right)^{-1} X^T\vec{y}}
\end{align*}

Note that $X^TX$ is positive semi-definite, and adding $\frac{\sigma^2}{\eta^2}I$ makes the whole matrix $X^TX + \frac{\sigma^2}{\eta^2}I$  positive-definite and thus invertible. 

\end{answer}
