\begin{answer}
\def\xsi{x^{(i)}}
We start with the PDF of the Laplace distribution, denoted  $g'(s) = \frac{1}{2}\exp(-|s|)$. Applying this into the likelihood given a single example $\xsi$, we get:

\begin{align*}
    \ell(W) &= \log|W| + \sum_{j=1}^\di \log \exp\left(-|w_j^T\xsi|)\right) \\
    &= \log|W| -\sum_{j=1}^\di |w_j^T\xsi| \\
    \Rightarrow \nabla_W\ell(W) &= W^{-T} - \begin{bmatrix} \nabla_{w_1}|w_1^T\xsi| \\ \nabla_{w_2}|w_2^T\xsi| \\
    \ldots \\
    \nabla_{w_{\di}}|w_{\di}^T\xsi|
    \end{bmatrix} \\
    &=  W^{-T} - \begin{bmatrix} \text{sign}(w_1^T\xsi)x^{(i)T} \\
    \text{sign}(w_2^T\xsi)x^{(i)T} \\
    \ldots\\
    \text{sign}(w_{\di}^T\xsi)x^{(i)T}
    \end{bmatrix} \\
    &= W^{-T} - \begin{bmatrix} \text{sign}(w_1^T\xsi) \\
    \text{sign}(w_2^T\xsi) \\
    \ldots\\
    \text{sign}(w_{\di}^T\xsi)
    \end{bmatrix}x^{(i)T}
\end{align*}

Resulting in the update rule:
\begin{align*}
    W := W + \alpha \left(W^{-T} - \begin{bmatrix} \text{sign}(w_1^T\xsi) \\
    \text{sign}(w_2^T\xsi) \\
    \ldots\\
    \text{sign}(w_{\di}^T\xsi)
    \end{bmatrix}x^{(i)T} \right)
\end{align*}
\end{answer}
