\begin{answer}
\begin{align*}
  p(t^{(i)}=1|y^{(i)}=1,x^{(i)})&=\dfrac{p(y^{(i)}=1|t^{(i)}=1,x^{(i)})p(t^{(i)}=1|x^{(i)})}{p(y^{(i)}=1|x^{(i)})}\\
  &=\dfrac{p(y^{(i)}=1|t^{(i)}=1,x^{(i)})p(t^{(i)}=1|x^{(i)})}{p(y^{(i)}=1|t^{(i)}=0,x^{(i)})p(t^{(i)}=0|x^{(i)}) +  p(y^{(i)}=1|t^{(i)}=1,x^{(i)})p(t^{(i)}=1|x^{(i)})}\\
  &=\dfrac{p(y^{(i)}=1|t^{(i)}=1,x^{(i)})p(t^{(i)}=1|x^{(i)})}{0 \cdot p(t^{(i)}=0|x^{(i)}) +  p(y^{(i)}=1|t^{(i)}=1,x^{(i)})p(t^{(i)}=1|x^{(i)})}\\
  &=\dfrac{p(y^{(i)}=1|t^{(i)}=1,x^{(i)})p(t^{(i)}=1|x^{(i)})}{p(y^{(i)}=1|t^{(i)}=1,x^{(i)})p(t^{(i)}=1|x^{(i)})}\\
  &=1
\end{align*}
\end{answer}
