\begin{answer}
  \begin{equation*}
      p(y;\eta) = \frac{b(y)e^{\eta y}}{\int b(y)e^{\eta y} dy}
\end{equation*}
\begin{equation*}
      A(\eta) = \int b(y)e^{\eta y} dy
\end{equation*}
\begin{equation*}
      a(\eta) = log A(\eta)
  \end{equation*}
  
  \begin{equation*}
      \frac{d}{d\eta}a(\eta) = \frac{d}{d\eta}log A(\eta)
  \end{equation*}
  \begin{equation*}
      = \frac{\frac{d}{d\eta}\int b(y)e^{\eta y} dy}{A(\eta)}  
  \end{equation*}
  By using hint in this sub-problem, we get...
  \begin{equation*}
      \frac{\int b(y)*y*e^{\eta y} dy}{A(\eta)} = \int\frac{ b(y)*y*e^{\eta y} dy}{A(\eta)} = \int p(y;\eta)y dy = E[Y;\eta]
  \end{equation*}
  Therefore, $E[Y;\eta] = \frac{d}{d\eta}a(\eta)$
\end{answer}
