\begin{answer}
We can find the Hessian $\nabla_{\theta'}^2 \log p(y;\theta')$ element-wise, as follows:
\newcommand{\dti}{\partial \theta'_i}
\newcommand{\dtj}{\partial \theta'_j}
\begin{align*}
\left[ \nabla_{\theta'}^2 \log p(y;\theta') \right]_{ij}
&= \frac{\partial^2 \log p(y;\theta')}{\dti \dtj}
= \frac{\partial}{\dtj} \frac{\partial \log p(y;\theta')}{\dti}
= \frac{\partial}{\dtj} \left[ \frac{1}{p(y;\theta')} \frac{\partial p(y;\theta')}{\dti} \right] \\
&= \frac{1}{p(y;\theta')} \frac{\partial^2 p(y;\theta')}{\dti \dtj} - \frac{1}{p(y;\theta')^2} \frac{\partial p(y;\theta')}{\dti} \frac{\partial p(y;\theta')}{\dtj} \\
&= \frac{1}{p(y;\theta')} \frac{\partial^2 p(y;\theta')}{\dti \dtj} - \frac{\partial \log p(y;\theta')}{\dti} \frac{\partial \log p(y;\theta')}{\dtj} \\
\nabla_{\theta'}^2 \log p(y;\theta')
&= \frac{\nabla_{\theta'}^2 p(y;\theta')}{p(y;\theta')} - \nabla_{\theta'} \log p(y;\theta') \nabla_{\theta'} \log p(y;\theta')^\top
\end{align*}

Alternatively, we can also find the Hessian in vector form as follows:
\begin{align*}
\nabla_{\theta'}^2 \log p(y;\theta')
&= \mathcal{J}_{\theta'} \left( \dfrac{\nabla_{\theta'} p(y;\theta')}{p(y;\theta')} \right) \quad\quad \text{where $\mathcal{J}$ denotes the Jacobian} \\
&= \dfrac{p(y;\theta') \nabla_{\theta'}^2 p(y;\theta')-\nabla_{\theta'} p(y;\theta') \nabla_{\theta'} p(y;\theta')^\top}{p(y;\theta')^2} \\
&= \dfrac{\nabla^2_{\theta'} p(y;\theta')}{p(y;\theta')} - \left( \dfrac{\nabla_{\theta'} p(y;\theta')}{p(y;\theta')} \right)\left( \dfrac{\nabla_{\theta'} p(y;\theta')}{p(y;\theta')} \right)^\top \\
&= \dfrac{\nabla_{\theta'}^2 p(y;\theta')}{p(y;\theta')} - \nabla_{\theta'} \log p(y;\theta') \nabla_{\theta'} \log p(y;\theta')^\top
\end{align*}

We now evaluate the following:
\begin{align*}
\E_{y \sim p(y;\theta)} \left[ \left. \dfrac{\nabla_{\theta'}^2 p(y;\theta')}{p(y;\theta')} \right|_{\theta'=\theta}\right]
&= \int_{-\infty}^\infty \dfrac{\nabla_{\theta'}^2 p(y;\theta')|_{\theta'=\theta}}{p(y;\theta')|_{\theta'=\theta}} p(y;\theta) dy \\
&= \int_{-\infty}^\infty \nabla_{\theta'}^2 p(y;\theta')|_{\theta'=\theta} dy \\
&= \nabla_{\theta'}^2 \left[ \int_{-\infty}^\infty p(y;\theta') dy \right]_{\theta'=\theta} \\
&= \nabla_{\theta'}^2 1|_{\theta'=\theta} \quad\quad \text{since $p(y;\theta')$ is a density function} \\
&= 0
\end{align*}

Evaluating limits on the first result and using our answer from part (b), we have
\begin{align*}
&\E_{y\sim \log p(y;\theta)}[-\nabla_{\theta'}^2 p(y;\theta')|_{\theta'=\theta}] \\
&= - \E_{y \sim p(y;\theta)} \left[ \left. \dfrac{\nabla_{\theta'}^2 p(y;\theta)}{p(y;\theta')} \right|_{\theta'=\theta}\right] + \E_{y \sim p(y;\theta)} \left[ \left. \nabla_{\theta'} \log p(y;\theta') \nabla_{\theta'} \log p(y;\theta')^\top \right|_{\theta'=\theta}\right] \\
&= 0 + \mathcal{I}(\theta)
= \mathcal{I}(\theta)
\end{align*}
\end{answer}
