\begin{answer}
  \begin{equation*}
      p(t^{i}=1|y^{i} = 1,x^{i}) = \frac{p(t^{i} = 1, y^{i} = 1, x^{i})}{p(y^{i} = 1, x^{i})}
  \end{equation*}
  \begin{equation*}
      = \frac{p(y^{i} = 1 |t^{i}=1,x^{i})p(t^{i}=1|x^{i})p(x^{i})}{p(y^{i} = 1 |t^{i}=1,x^{i})p(t^{i}=1|x^{i})p(x^{i}) + p(y^{i} = 1 |t^{i}=0,x^{i})p(t^{i} = 0|x^{i})p(x^{i})}
  \end{equation*}
  \begin{equation*}
      = \frac{\alpha*p(t^{i} = 1|x^{i})}{0 + \alpha*p(t^{i} = 1|x^{i})} = \frac{\alpha*p(t^{i} = 1|x^{i})}{\alpha*p(t^{i} = 1|x^{i})} = 1
  \end{equation*}
  
  Therefore, 
  \begin{equation*}
p(t^{(i)}=1\mid y^{(i)} = 1, x^{(i)}) = 1
\end{equation*}
\end{answer}
