\begin{answer}
\begin{align*}
-\KL(P\|Q) &= -\sum_x P(x)\log\frac{P(x)}{Q(x)}\\
&= \sum_x P(x)\log\frac{Q(x)}{P(x)}\\
&\leq \log \sum_x P(x)\frac{Q(x)}{P(x)}\\
&= \log \sum_x Q(x)\\
&= \log 1 \\
&= 0
\end{align*}
Where all equalities follow from straight forward algebraic
manipulation. The inequality follows from Jensen's inequality.

To show the second part of the claim, note that $\log t$ is a
strictly concave function of $t$.  Using the form of Jensen's
inequality given in the lecture notes, we have
equality if and only if
$\frac{Q(x)}{P(x)}=\E_P \left[\frac{Q(x)}{P(x)}\right]$
for all $x$.  But since
$\E_P \left[\frac{Q(x)}{P(x)}\right] = \sum_x P(x) \frac{Q(x)}{P(x)} = \sum_x Q(x) = 1$,
it follows that
$P(x)=Q(x)$. Hence we have $\KL(P\|Q)=0$ if and only if
$P(x)=Q(x)$ for all $x$.
\end{answer}
